src/theory/bir/bir_mem_coreScript.sml
@@ -15,7 +15,7 @@ mem_state_t = <|
 (*  bmst_status   : bir_status_t; *)
   bmst_lock     : num option;
   bmst_counter  : num;
-  bmst_inflight : (string bir_inflight_stmt_t) list
+  bmst_inflight : (num # string bir_inflight_stmt_t) list
   |>
 `;
 
@@ -27,7 +27,7 @@ memfresh s = STRCAT "mt" (n2s s.bmst_counter)
 val next_memop_def = Define`
 next_memop s = case s.bmst_inflight of
                    [] => NONE
-                 | ((BirInflight t0 stm)::stms) => SOME (t0,stm)
+                 | ((cid,BirInflight t0 stm)::stms) => SOME (t0,stm)
 `;
 
 val commit_memop_def = Define`
@@ -40,10 +40,23 @@ case bir_eval_exp ex s.bmst_environ of
      | NONE => ARB
 `;
 
+val memflush_def = Define`
+   (memflush target_cid [] s = s)
+/\ (memflush target_cid ((cid,BirInflight t0 stm)::stms) s =
+    if cid = target_cid
+    then memflush target_cid stms (commit_memop stm s)
+    else memflush target_cid stms s)
+`;
+
+val remove_mem_inflight_def = Define`
+remove_mem_inflight t l =
+   FILTER (\bi . case bi of (_,BirInflight t0 _) => (t <> t0)) l
+`;
+
 val (memstep_rules, memstep_ind, memstep_cases) = Hol_reln`
 (!s1 s2 stm. ((next_memop s1 = SOME (t0,stm))
               /\ (commit_memop stm s1 = s2))
-     ==> memstep s1 (s2 with bmst_inflight updated_by (remove_inflight t0)))
+     ==> memstep s1 (s2 with bmst_inflight updated_by (remove_mem_inflight t0)))
 `;
 
 val mem_compute_next_def = Define`
@@ -51,7 +64,7 @@ val mem_compute_next_def = Define`
         case next_memop ms of
             NONE => []
           | SOME (t0,stm) =>
-            [commit_memop stm ms with bmst_inflight updated_by (remove_inflight t0)]
+            [commit_memop stm ms with bmst_inflight updated_by (remove_mem_inflight t0)]
 `;
 
 val mem_init_def = Define`
